theories/logic/satisfiable.v
@@ -1,0 +1,99 @@
+From iris Require Import bi bi.lib.fixpoint bi.updates bi.derived_laws.
+From iris.proofmode Require Import tactics.
+Import bi.
+
+(* Satisfiability *)
+Section satisfiable.
+
+  Context {PROP : bi}.
+  Context {PROP_bupd : BiBUpd PROP}.
+  Context {PROP_affine : BiAffine PROP}.
+  Implicit Types (P Q: PROP).
+
+  Class Satisfiable (sat: PROP → Prop) := {
+    sat_mono P Q: (P ⊢ Q) → sat P → sat Q;
+    sat_elim φ: sat (⌜φ⌝)%I → φ;
+    sat_bupd P: sat (|==> P)%I → sat P;
+    sat_exists {X} Φ: sat (∃ x: X, Φ x)%I → ∃ x: X, sat (Φ x);
+  }.
+
+  Section derived_lemmas.
+    Context {sat: PROP → Prop} `{Satisfiable sat}.
+    Arguments sat _%I.
+
+    (* derived *)
+    Global Instance sat_if: Proper ((⊢) ==> impl) sat.
+    Proof. intros P Q Hent Hsat; by eapply sat_mono. Qed.
+
+    Global Instance sat_equiv: Proper ((≡) ==> iff) sat.
+    Proof.
+      intros P Q Heq; split; intros Hsat; eauto using sat_mono, equiv_entails, equiv_entails_sym.
+    Qed.
+
+    Lemma sat_sep P Q: sat (P ∗ Q) → sat P ∧ sat Q.
+    Proof.
+      intros Hsat; split; eapply sat_mono, Hsat; by iIntros "[P Q]".
+    Qed.
+    Lemma sat_and P Q: sat (P ∧ Q) → sat P ∧ sat Q.
+    Proof.
+      intros Hsat; split; eapply sat_mono, Hsat;
+      eauto using bi.and_elim_l, bi.and_elim_r.
+    Qed.
+    Lemma sat_or P Q: sat (P ∨ Q) → sat P ∨ sat Q.
+    Proof.
+      rewrite or_alt; intros [[] Hsat] % sat_exists; eauto.
+    Qed.
+    Lemma sat_forall {X} Φ x: sat (∀ x: X, Φ x) → sat (Φ x).
+    Proof.
+      eapply sat_mono; eauto.
+    Qed.
+    Lemma sat_pers P: sat (<pers> P) → sat P.
+    Proof.
+      eapply sat_mono; eauto.
+    Qed.
+    Lemma sat_intuitionistic P: sat (□ P) → sat P.
+    Proof.
+      eapply sat_mono; eauto.
+    Qed.
+    Lemma sat_impl P Q: (⊢ P) → sat (P → Q) →  sat Q.
+    Proof.
+      intros Hent Hsat; eapply sat_mono, Hsat.
+      iIntros "H". iApply impl_elim_r. iSplit; eauto.
+      iApply Hent.
+    Qed.
+    Lemma sat_wand P Q: (⊢ P) → sat (P -∗ Q) → sat Q.
+    Proof.
+      intros Hent Hsat; eapply sat_mono, Hsat.
+      iIntros "HPQ". iApply "HPQ". iApply Hent.
+    Qed.
+  End derived_lemmas.
+
+  Section sat_frame.
+    Context {sat: PROP → Prop} `{Satisfiable sat}.
+    Arguments sat _%I.
+
+    Definition sat_frame (F P: PROP) := sat (F ∗ P).
+
+    Global Instance sat_frame_satisfiable F: Satisfiable (sat_frame F).
+    Proof.
+      split; unfold sat_frame.
+      - intros P Q HPQ Hsat. eapply sat_mono, Hsat.
+        iIntros "($ & P)". by iApply HPQ.
+      - intros Φ Hsat. eapply sat_elim, sat_mono, Hsat.
+        iIntros "(_ & $)".
+      - intros P Hsat. eapply sat_bupd, sat_mono, Hsat.
+        iIntros "($ & $)".
+      - intros X Φ Hsat. eapply sat_exists, sat_mono, Hsat.
+        iIntros "($ & $)".
+    Qed.
+
+    Lemma sat_frame_intro P F Q:
+      (P -∗ F ∗ Q) → sat P → sat_frame F Q.
+    Proof.
+      unfold sat_frame; eapply sat_mono.
+    Qed.
+
+  End sat_frame.
+
+End satisfiable.
+Arguments sat_frame {_} {_}%function_scope _%I _%I.
